test-suite/erasure_live_test.v
@@ -1,5 +1,7 @@
 From Coq Require Import Recdef.
 From MetaCoq.Template Require Import Loader.
+From MetaCoq.SafeChecker Require Import SafeTemplateChecker.
+From MetaCoq.PCUIC Require Import PCUICAstUtils.
 From MetaCoq.Erasure Require Import Erasure.
 From Coq Require Import String.
 Local Open Scope string_scope.
@@ -10,6 +12,26 @@ Definition test (p : Ast.program) : string :=
   erase_and_print_template_program p.
 
 MetaCoq Quote Recursively Definition zero := 0.
+
+(* Definition zerocst_test : ∑ s, test zero = s.
+Proof.
+  eexists.
+  unfold test, erase_and_print_template_program.
+  set(e := fix_program_universes zero).
+  cbn in e.
+  unfold erase_template_program.
+  set (foo := ErasureFunction.erase _ _ _ _ _).
+  hnf in foo.
+  unfold ErasureFunction.is_erasable in foo.
+  set (isa := ErasureFunction.is_arity _ _ _ _ _ _) in *.
+  hnf in isa.
+  set (rs := PCUICTypeChecker.reduce_to_sort _ _ _ _) in *.
+  elimtype False. clear foo isa.
+  hnf in rs.
+
+
+  simpl in foo. *)
+
 Definition zerocst := Eval lazy in test zero.
 
 MetaCoq Quote Recursively Definition exproof := I.
